Automata/Projection.lean
@@ -1,11 +1,15 @@
 import Mathlib.Tactic
 import Mathlib.Data.List.Basic
+import Batteries.Data.List.Basic
 import Mathlib.Data.Nat.Digits
 import Automata.DFA
 import Automata.NFA
+import Automata.Pumping
 import Automata.Input
 import Automata.Addition
 import Automata.Replicate
+import Automata.Collapse
+import Automata.Vector
 
 
 -- Auxilliary theorems for recover
@@ -14,19 +18,22 @@ theorem finLt (m : Fin (n+1)) (b : ℕ) : b < m.val → b < n := by omega
 theorem finPred (m : Fin n) (a : Fin n) (h : a > m): a.val - 1 < n - 1 := by omega
 
 -- Auxilliary function for project
-def recover (m : Fin (n + 1)) (x: Fin (b+2)):
-  (Fin n → Fin (b+2)) → (Fin (n + 1) → Fin (b+2)) :=
-    fun i => fun j => if h1: j.val < m.val then i ⟨j.val, finLt m j.val h1⟩
-      else if h2: j.val > m.val then i ⟨j.val - 1, finPred m j h2⟩ else x
+def recover_value (m : Fin (n + 1)) (x: Fin (b+2)) (f: Fin n → Fin (b+2)) :
+ (Fin (n + 1) → Fin (b+2)) :=
+    fun i => if h1: i.val < m.val then f ⟨i.val, finLt m i.val h1⟩
+      else if h2: i.val > m.val then f ⟨i.val - 1, finPred m i h2⟩ else x
 
 def project (m : Fin (n+1)) (dfa : DFA (Fin (n+1) → Fin (b+2)) state) [DecidableEq state] :
   NFA (Fin n → Fin (b+2)) state := {
   transition :=
-  fun a q => ⟨(List.map (fun (x : Fin (b+2)) => dfa.transition (recover m x a) q)
+  fun a q => ⟨(List.map (fun (x : Fin (b+2)) => dfa.transition (recover_value m x a) q)
     (FinEnum.toList (Fin (b+2)))).dedup, by apply List.nodup_dedup⟩
   start := ⟨[dfa.start], List.nodup_singleton dfa.start⟩
   output := dfa.output
 }
+
+theorem project_accept [DecidableEq state](dfa : DFA (Fin (n + 1) → Fin (b+2)) state) (m : Fin (n + 1)) (l : List (Fin n → Fin (b+2))) : dfa.eval (l.map (recover_value m x)) → (project m dfa).eval l := by
+  sorry
 
 #eval [(fun _ => 0 : Fin 2 → Fin (0 + 2)), fun _ => 1]
 -- Problem: exists x, 1 + 1 = x?
@@ -35,6 +42,14 @@ def project (m : Fin (n+1)) (dfa : DFA (Fin (n+1) → Fin (b+2)) state) [Decidab
 #eval (project 2 (addBase 2)).eval [fun _ => 0, fun _ => 1]
 
 #eval (project 2 (addBase 2)).eval (inputToBase 2 (by omega) [100000, 10000])
+
+-- Exists x, y + x = x?
+#eval (project 1 (collapse 2 1 (addBase 2))).eval (inputToBase 2 (by omega) [100000])
+
+#eval (project 1 (collapse 2 1 (addBase 2))).eval (inputToBase 2 (by omega) [10])
+
+-- Exists x, x + x = x?
+#eval (project 0 (collapse 1 0 (collapse 2 1 (addBase 2)))).eval (inputToBase 2 (by omega) [])
 
 def padZeroes (m : ℕ) (x : List (Fin n → Fin (b+2))) : List (Fin n → Fin (b+2)) :=
   List.replicate m (fun _ => 0) ++ x
@@ -56,6 +71,16 @@ theorem padZeroes_diff (a b: ℕ) (x y : List (Fin n → Fin (k+2))) (hab : a �
   apply List.eq_diff_of_replicate_append_eq
   . exact h
   . exact hab
+
+def DFA.acceptZero (dfa : DFA (Fin n → Fin (b+2)) state) : Prop := ∀ (x : List (Fin n → Fin (b+2))), dfa.eval x → (∀ m, dfa.eval (padZeroes m x))
+
+def NFA.acceptZero [DecidableEq state] (nfa : NFA (Fin n → Fin (b+2)) state) : Prop := ∀ (x : List (Fin n → Fin (b+2))), nfa.eval x → (∀ m, nfa.eval (padZeroes m x))
+
+theorem project_acceptZero [DecidableEq state] (dfa : DFA (Fin (n + 1) → Fin (b+2)) state) (h: DFA.acceptZero dfa) (m : Fin (n + 1)) : NFA.acceptZero (project m dfa) := by
+  simp only [DFA.acceptZero, NFA.acceptZero] at *
+  intro x hx z
+  simp only [project, NFA.eval, NFA.transFrom, recover_value]
+  sorry
 
 theorem DFAO.bounded_out [Fintype state] (dfao : DFAO (Fin n → Fin (b+2)) state out) (x : List (Fin n → Fin (b+2))) (o: out)(h: ∀ (x : List (Fin n → Fin (b+2))), dfao.eval x = o → (∀ m, dfao.eval (padZeroes m x) = o)) : ∀ k, dfao.eval (padZeroes k x) = o → dfao.eval (padZeroes (Fintype.card state) x) = o := by
   rintro k hkxo
@@ -159,18 +184,18 @@ theorem DFAO.bounded_out [Fintype state] (dfao : DFAO (Fin n → Fin (b+2)) stat
       . exact hkb
       . rfl
 
-theorem DFA.bounded_accept [Fintype state] (dfa : DFA (Fin n → Fin (b+2)) state) (x : List (Fin n → Fin (b+2)))(h: ∀ (x : List (Fin n → Fin (b+2))), dfa.eval x→ (∀ m, dfa.eval (padZeroes m x))): ∀ z, (∃ k, z = padZeroes k x) ∧ dfa.eval z → dfa.eval (padZeroes (Fintype.card state) x) := by
+theorem DFA.bounded_accept [Fintype state] (dfa : DFA (Fin n → Fin (b+2)) state) (x : List (Fin n → Fin (b+2)))(h: dfa.acceptZero): ∀ z, (∃ k, z = padZeroes k x) ∧ dfa.eval z → dfa.eval (padZeroes (Fintype.card state) x) := by
   have := DFAO.bounded_out dfa x true
   intro z a
-  simp_all only [implies_true, true_implies]
+  simp_all only [implies_true, true_implies, DFA.acceptZero]
   obtain ⟨left, right⟩ := a
   obtain ⟨w, h_1⟩ := left
   subst h_1
   apply this
   · exact right
 
-theorem NFA.bounded_accept [Fintype state] [DecidableEq state] (nfa : NFA (Fin n → Fin (b+2)) state) (x : List (Fin n → Fin (b+2)))(h: ∀ (x : List (Fin n → Fin (b+2))), nfa.eval x→ (∀ m, nfa.eval (padZeroes m x))): ∀ z, (∃ k, z = padZeroes k x) ∧ nfa.eval z → nfa.eval (padZeroes (Fintype.card (ListND state)) x) := by
-  simp only [← NFA.toDFA_eval] at *
+theorem NFA.bounded_accept [Fintype state] [DecidableEq state] (nfa : NFA (Fin n → Fin (b+2)) state) (x : List (Fin n → Fin (b+2)))(h: nfa.acceptZero): ∀ z, (∃ k, z = padZeroes k x) ∧ nfa.eval z → nfa.eval (padZeroes (Fintype.card (ListND state)) x) := by
+  simp only [NFA.acceptZero, ← NFA.toDFA_eval] at *
   have := DFA.bounded_accept (nfa.toDFA) x h
   intro z a
   simp_all only [and_imp, forall_exists_index]
@@ -181,146 +206,6 @@ theorem NFA.bounded_accept [Fintype state] [DecidableEq state] (nfa : NFA (Fin n
   · rfl
   · exact right
 
-
-
--- Old version
--- theorem DFAO.bounded_out [Fintype state] (dfao : DFAO (Fin n → Fin (b+2)) state out) (x : List (Fin n → Fin (b+2))) (o: out)(h: ∀ (x : List (Fin n → Fin (b+2))), dfao.eval x = o → (∀ y, (∃ m, y = padZeroes m x) →  dfao.eval y = o)) : ∀ z, (∃ k, z = (padZeroes k x)) ∧ dfao.eval z = o → dfao.eval (padZeroes (Fintype.card state) x) = o := by
---   simp only [padZeroes]
---   rintro z ⟨⟨k, hz⟩, hzo⟩
---   by_cases hkstate : k ≤ Fintype.card state
---   . apply h z
---     . exact hzo
---     . use Fintype.card state - k
---       rw[hz]
---       simp only [padZeroes]
---       rw[← List.append_assoc, ← List.replicate_add]
---       subst hzo hz
---       simp only [List.append_cancel_right_eq, List.replicate_inj, or_true, and_true]
---       omega
-
---   simp only [not_le] at hkstate
---   -- Question: How to get this kind of descent argument work in lean?
---   . induction' hk : k - Fintype.card state using Nat.strong_induction_on  with d ih generalizing k z
---     have hzlen : Fintype.card state ≤ z.length := by
---       rw[hz]
---       simp only [List.length_append, List.length_replicate]
---       omega
-
---     obtain ⟨a, b', c, hzabc, hablen, hne, hy⟩ := dfao.pumping_lemma_eval hzo hzlen
---     have haco : dfao.eval (a ++ c) = o := by
---       apply hy
---       simp only [Language.mem_mul, exists_exists_and_exists_and_eq_and, List.append_assoc]
---       use a, (by exact rfl), [], (by exact Language.nil_mem_kstar {b'}), c, (by exact rfl)
---       simp only [List.nil_append]
---     -- have hblen : 0 < b'.length := by
---     --   exact List.length_pos_of_ne_nil hne
-
---     have habzero' : ∀ i, ∀ (hi: i < a.length + b'.length),  z[i]'(by omega) = fun _ => 0 := by
---       intro i hi
---       have hik : i < k := by
---         omega
---       simp only [hz]
---       rw[List.getElem_append_left, List.getElem_replicate]
---       rwa[List.length_replicate]
---     have habzero : ∀ i, ∀ (hi: i < a.length + b'.length),  (a ++ b')[i]' (by rw[List.length_append]; exact hi) = fun _ => 0 := by
---       intro i hi
---       rw[← List.getElem_append_left (a++b') c]
---       trans z[i]
---       . congr; exact hzabc.symm
---       specialize habzero' i hi
---       convert habzero'
---       simp only [List.append_assoc, List.length_append]
---       . omega
-
---     have hazero : ∀ i, ∀ (hi: i < a.length),  a[i]' (by omega) = fun _ => 0 := by
---       intro i hi
---       rw[← List.getElem_append_left a b']
---       apply habzero i
---       . omega
---     have hbzero : ∀ i, ∀ (hi: i < b'.length),  b'[i]' (by omega) = fun _ => 0 := by
---       intro i hi
---       -- rw[← List.getElem_append_right' a b'] Why?
---       have : (a ++ b')[a.length + i]'(by rw[List.length_append]; omega) = b'[i] := by
---         rw[List.getElem_append_right']
---         simp only [add_tsub_cancel_left]
---         omega
---       rw[← this]
---       apply habzero (a.length + i)
---       omega
---     have har: a = List.replicate a.length (fun _ => 0) := by
---       apply List.ext_getElem
---       . simp
---       . intro n_1 h₁ h₂
---         simp only [List.getElem_replicate]
---         exact hazero n_1 h₁
---     have hbr: b' = List.replicate b'.length (fun _ => 0) := by
---       apply List.ext_getElem
---       . simp
---       . intro n_1 h₁ h₂
---         simp only [List.getElem_replicate]
---         exact hbzero n_1 h₁
---     have habk : a.length + b'.length < k := by omega
---     have hk : (List.replicate k (fun _ => 0)) = (List.replicate (a.length + b'.length) (fun _ => 0)) ++ (List.replicate (k - a.length - b'.length) (fun _ : Fin n => (0 : Fin (b + 2)))) := by
---       simp[List.append_replicate_replicate]
---       omega
---     have hcx : c = (List.replicate (k - a.length - b'.length) (fun _ => 0)) ++ x := by
---       rw[har, hbr] at hzabc
---       rw[hzabc] at hz
---       simp only [List.append_replicate_replicate] at hz
---       -- AHhhh! NO!
---       rw[hk] at hz
---       rw[List.append_assoc] at hz
---       exact List.append_cancel_left hz
-
---     have hac : a ++ c = List.replicate (k - b'.length) (fun _ => 0) ++ x := by
---       rw[hcx, har]
---       rw[← List.append_assoc]
---       simp only [List.length_replicate, List.append_replicate_replicate,
---         List.append_cancel_right_eq, List.replicate_inj, AddLeftCancelMonoid.add_eq_zero,
---         List.length_eq_zero, or_true, and_true]
---       omega
---     by_cases hkb : k - b'.length ≤ Fintype.card state
---     . apply h (a ++ c)
---       . exact haco
---       . -- subst/rw hac !!!
---         use Fintype.card state - (k - b'.length)
---         simp only [hac, padZeroes]
---         rw[← List.append_assoc]
---         simp only [List.append_replicate_replicate, List.append_cancel_right_eq, List.replicate_inj,
---           or_true, and_true]
---         omega
---     . simp only [not_le] at hkb
---       have hblen : 0 < b'.length := by
---         exact List.length_pos_of_ne_nil hne
-
---       specialize ih (k - b'.length - Fintype.card state) (by omega) (a ++ c) (haco) (k - b'.length) hac hkb rfl
-
---       exact ih
-
--- theorem DFA.bounded_accept [Fintype state] (dfa : DFA (Fin n → Fin (b+2)) state) (x : List (Fin n → Fin (b+2)))(h: ∀ (x : List (Fin n → Fin (b+2))), dfa.eval x→ (∀ y, (∃ m, y = padZeroes m x) →  dfa.eval y)) : ∀ z, (∃ k, z = padZeroes k x) ∧ dfa.eval z → dfa.eval (padZeroes (Fintype.card state) x) := by
---   have := DFAO.bounded_out dfa x true
---   intro z a
---   simp_all only [forall_exists_index, and_imp]
---   obtain ⟨left, right⟩ := a
---   obtain ⟨w, h_1⟩ := left
---   subst h_1
---   apply this
---   · intro x_1 a y x_2 h_1
---     subst h_1
---     apply h
---     · simp_all only
---     · rfl
---   · rfl
---   · exact right
-
--- theorem NFA.bounded_accept [Fintype state] [DecidableEq state] (nfa : NFA (Fin n → Fin (b+2)) state) (x : List (Fin n → Fin (b+2)))(h: ∀ (x : List (Fin n → Fin (b+2))), nfa.eval x→ (∀ y, (∃ m, y = padZeroes m x) →  nfa.eval y)) : ∀ z, (∃ k, z = padZeroes k x) ∧ nfa.eval z → nfa.eval (padZeroes (Fintype.card (ListND state)) x) := by
---   simp only [← NFA.toDFA_eval] at *
---   have := DFA.bounded_accept (nfa.toDFA) x h
---   intro z a
---   simp_all only [forall_exists_index, and_imp]
---   obtain ⟨left, right⟩ := a
---   obtain ⟨w, h_1⟩ := left
---   subst h_1
---   apply this
---   · rfl
---   · exact right
+theorem project_correct [Fintype state] [DecidableEq state] (l : List ℕ) (m : Fin (l.length + 1)) (dfa : DFA (Fin (l.length +1) → Fin (b+2)) state) (h: dfa.acceptZero):
+  ∃ (x : ℕ), dfa.eval (dcast (by congr; apply List.length_insertNth; exact Fin.is_le m) (inputToBase (b+2) (by omega) (l.insertNth m x))) ↔ (project m dfa).eval (padZeroes (Fintype.card (ListND state)) (inputToBase (b+2) (by omega) l)):= by
+  sorry
