.vscode/UselessFIles/Equality_Fin.lean
@@ -1,0 +1,88 @@
+import Mathlib.Tactic
+import Mathlib.Data.List.Basic
+import Automata.DFA_Fin
+import Automata.Input_Fin
+
+def eqBase (k: ℕ) : DFA (Fin 2 → Fin k) (Fin 2) := {
+  transition := fun f s => match s with
+    | 0 => if (f 0).val = f 1 then 0 else 1
+    | 1 => 1
+  start := 0
+  output := fun x => x == 0
+}
+
+theorem eqBase_if_equal_aux (b : ℕ) (f: Fin n → Fin 2 → Fin b) :
+  (∀ (x : Fin n), ((f x) 0).val = (f x) 1) → (eqBase b).evalFrom f 0 := by
+  intro h
+  induction n
+  case zero =>
+    simp_all only [Fin.isValue, IsEmpty.forall_iff]
+    rfl
+  case succ n ih =>
+    simp[DFAO.evalFrom, DFAO.transFrom]
+    have : ((eqBase b).transition (f 0) 0) = 0 := by
+      simp[eqBase]; exact h 0
+    rw[this]
+    specialize ih (Fin.tail f)
+    apply ih
+    intro x
+    apply h
+
+example (b : ℕ) (f: Fin n → Fin 2 → Fin b) :
+  (∀ (x : ℕ) (hx: x < n), ((f ⟨x, hx⟩) 0).val = (f ⟨x, hx⟩) 1) → (eqBase b).evalFrom f 0 := by
+  intro h
+  induction n
+  case zero =>
+    simp_all only [Fin.isValue, IsEmpty.forall_iff]
+    rfl
+  case succ n ih =>
+    simp[DFAO.evalFrom, DFAO.transFrom]
+    have : ((eqBase b).transition (f 0) 0) = 0 := by
+      simp[eqBase]; apply h 0
+    rw[this]
+    specialize ih (Fin.tail f)
+    apply ih
+    intro x
+    specialize h (x + 1)
+    intro hxn
+    simp[Fin.tail]
+    apply h
+
+
+theorem eqBase_trans_zero (k : ℕ) (state : Fin 2) (f : Fin 2 → Fin k) :
+  (eqBase k).transition f state = 0 ↔ state = 0 ∧ (f 0).val = f 1 := by
+  simp only [eqBase, Fin.isValue, beq_iff_eq]
+  split <;> simp
+
+theorem eqBase_transFrom_zero (k : ℕ) (state: Fin 2) (f : Fin n → Fin 2 → Fin k) :
+  (eqBase k).transFrom f state = 0 ↔ state = 0 ∧ ∀ (x : Fin n), ((f x) 0).val = f x 1 := by
+  induction n generalizing state
+  case zero =>
+    simp_all only [Fin.isValue, IsEmpty.forall_iff, and_true]
+    rfl
+  case succ n ih =>
+    simp[DFAO.transFrom]
+    specialize ih ((eqBase k).transition (f 0) state) (Fin.tail f)
+    rw[ih]
+    constructor
+    . intro h
+      rcases h with ⟨h1, h2⟩
+      have:= (eqBase_trans_zero k state (f 0)).mp h1
+      rcases this with ⟨rfl, h⟩
+      simp only [Fin.isValue, true_and]
+      intro x
+      by_cases hx: x = 0 -- x.val = 0 also won't work
+      . rw[hx]
+        exact h
+      . specialize h2 ⟨x.val - 1, by omega⟩
+        simp[Fin.tail] at h2
+        have : x.val ≠ 0 := by
+          intro h'
+          apply hx
+          exact Eq.symm (Fin.eq_of_val_eq (id (Eq.symm h')))
+        -- cases' x with x
+        -- .
+        -- doesn't work have : ¬ x.val = 0 := by omega
+        have h3: x.val - 1 + 1 = x.val := by omega
+        simp_all only [Fin.isValue, true_and, Fin.eta, ne_eq]
+    . sorry
