.vscode/UselessFIles/Input_Fin.lean
@@ -1,0 +1,94 @@
+import Mathlib.Tactic
+import Mathlib.Data.Nat.Digits
+
+def toBase (b : ℕ) (n : ℕ): List ℕ :=
+  (Nat.digits b n).reverse
+
+theorem digits_end_nonzero (b: ℕ) (n: ℕ) (hb: b ≥ 2) (hn : n > 0) :
+  (Nat.digits b n)[(Nat.digits b n).length - 1]'(by
+  simp[Nat.digits]
+  split <;> try simp at hb
+  rename_i x y
+  rw[Nat.digitsAux.eq_def]
+  split <;> try simp at hn
+  simp
+  ) > 0 := by
+  have:= Nat.digits_of_two_le_of_pos hb hn
+  induction' n using Nat.strong_induction_on with n ih
+  simp[this]
+  have h1: n / b < n := Nat.div_lt_self hn hb
+  by_cases hnb : n / b ≠ 0
+  have: n / b > 0 := by exact Nat.zero_lt_of_ne_zero hnb
+  specialize ih (n / b) h1 this
+  have := Nat.digits_of_two_le_of_pos hb this
+  specialize ih this
+  aesop
+  . simp at hnb
+    have: b.digits (n / b) = [] := by
+      rw[hnb]
+      apply Nat.digits_zero
+    simp[this]
+    have: n = b * (n / b) + n % b := by
+      exact Eq.symm (Nat.div_add_mod n b)
+    simp[hnb] at this
+    rw[← this]
+    exact hn
+
+theorem toBase_lead_nonzero (b: ℕ) (n: ℕ) (hb: b ≥ 2) (hn : n > 0) :
+  (toBase b n)[0]'(by
+  simp[toBase, Nat.digits]
+  split <;> try simp at hb
+  rw[Nat.digitsAux.eq_def]
+  split <;> try simp at hn
+  simp
+  ) > 0 := by
+  simp[toBase]
+  exact digits_end_nonzero b n hb hn
+
+theorem toBase_lt_base (b: ℕ) (n: ℕ) (hb: b ≥ 2) :
+  x ∈ (toBase b n) → x < b := by
+  intro h
+  simp only [toBase] at h
+  have h1: x ∈ Nat.digits b n := List.mem_reverse.mp h
+  apply Nat.digits_lt_base
+  exact hb
+  exact h1
+
+def toBase' (b: ℕ) (n: ℕ) (h : b ≥ 2): List (Fin b) :=
+  (toBase b n).attach.map (fun x => ⟨x.1, (by apply toBase_lt_base b n (by omega); obtain ⟨val, property⟩ := x; simp_all only)⟩)
+
+def toBaseFin (b n: ℕ) (h : b ≥ 2): Fin (toBase' b n h).length → Fin b :=
+  fun i => (toBase' b n h)[i]
+
+def stretchFin (m: ℕ) (h : b ≥ 2) (f : Fin n → Fin b) : Fin (m + n) → Fin b :=
+  fun i => if h1: i.val < m then ⟨0, by omega⟩ else f ⟨i.val - m, (by omega)⟩
+
+def stretchFinTo (m: ℕ) (h : b ≥ 2) (f : Fin n → Fin b) (hmn : m ≥ n) : Fin m → Fin b :=
+  fun i => if h1: i.val < m - n then ⟨0, by omega⟩ else f ⟨i.val - (m - n), (by omega)⟩
+
+def maxFin (b: ℕ) (l: List ℕ) (h: b ≥ 2) : ℕ :=
+  match l with
+    | [] => 0
+    | x::xs => max ((toBase' b x h).length) (maxFin b xs h)
+
+theorem maxFin_max (b: ℕ) (l: List ℕ) (h: b ≥ 2) : ∀ i, i ∈ l → maxFin b l h ≥ (toBase' b i h).length := by
+  intro i hi
+  induction l with
+    | nil => contradiction
+    | cons x xs ih =>
+      rcases hi with hi | hi
+      . simp only [maxFin, le_max_iff, le_refl, true_or]
+      . simp only [maxFin, le_max_iff]
+        right
+        rename_i a
+        apply ih
+        exact a
+
+def mapToBaseFin (b: ℕ) (l: List ℕ) (h: b ≥ 2): Fin l.length → Fin (maxFin b l h) → Fin b :=
+  fun i => (stretchFinTo (maxFin b l h) h (toBaseFin b l[i] h) (by apply maxFin_max; apply List.getElem_mem) : Fin (maxFin b l h) → Fin b)
+
+def toInputFin (b: ℕ) (l: List ℕ) (h: b ≥ 2): Fin (maxFin b l h) → Fin l.length → Fin b :=
+  fun i => fun j => mapToBaseFin b l h j i
+
+def padZero (k : ℕ) (f : Fin m → Fin n → Fin b) (h : b ≥ 2) : Fin (k + m) → Fin n → Fin b :=
+  fun i => fun j => if h: i.val < k then ⟨0, by omega⟩ else f ⟨i.val - k, (by omega)⟩ j
