Automata/Collapse.lean
@@ -1,0 +1,135 @@
+import Mathlib.Tactic
+import Automata.DFA
+import Automata.Input
+import Automata.Vector
+import Automata.Equality_Gen
+
+/-
+1. General Equality
+2. The Collapse Problem
+3. Fin operations? Mathlib weird
+4. Casting!
+5. Writeup?
+
+-/
+
+variable {α : Type} {n : ℕ} {b : ℕ}
+
+-- Auxilliary functions for collapse
+def tail (f: Fin (n+1) → α) : Fin n → α :=
+  fun i => f (i.succ)
+
+#check Fin.insertNth
+
+def remove_index (i : Fin (n + 1)) (f: Fin (n + 1) → α):
+   (Fin n → α) :=
+    fun j => f (if j.val < i.val then j else ⟨j.val + 1, by omega⟩)
+
+def recover_index (i : Fin (n + 1)) (k: Fin n) (f: Fin n → α):
+   (Fin (n + 1) → α) :=
+    fun j => if hlt : j < i then f ⟨j, by omega⟩ else if hgt : j > i then f ⟨j - 1, by omega⟩ else f k
+
+
+
+theorem remove_recover (i : Fin (n + 1)) (k: Fin n) (f: Fin n → α) :
+  remove_index i (recover_index i k f) = f := by
+  ext x
+  simp[remove_index, recover_index]
+  split; simp only [Fin.coe_castSucc, Fin.eta, dite_eq_ite, ite_eq_then, not_lt]
+  . intro h
+    have : i.val ≤ x.val := by exact h
+    omega
+  . split
+    . rename_i hsucc h
+      have : x.val + 1 < i.val := by
+        simp_all only [not_lt]
+        exact h
+      omega
+    . split
+      . rfl
+      . rename_i h₁ h₂ h₃
+        have : ¬ x.val + 1 < i.val := by
+          simp_all only [not_lt]
+          exact h₂
+        have : ¬ i.val < x.val + 1 := by
+          simp_all only [not_lt]
+          exact h₃
+        omega
+
+theorem recover_remove (i : Fin (n + 1)) (k: Fin n) (f: Fin (n + 1) → α) (hf: f i = f k) (hik : i.val > k.val ) :
+  recover_index i k (remove_index i f) = f := by
+  ext x
+  simp[remove_index, recover_index]
+  split; simp only [Fin.coe_castSucc, Fin.eta, dite_eq_ite, ite_eq_then, not_lt]
+  . split; simp_all
+    . split
+      .
+        -- have : i.val < x.val := by omega
+
+        omega
+      . rcases x with ⟨x, hx⟩
+        cases x; contradiction
+        rfl
+    . simp_all only [Fin.coe_eq_castSucc, gt_iff_lt, not_lt]
+      have : x = i := by omega
+      subst this
+      simp_all only [le_refl]
+
+def collapse (i : Fin (n+1)) (k : Fin n) (dfa : DFA (Fin (n+1) → α) state) : DFA (Fin n → α) state := {
+  transition := fun a q => dfa.transition (recover_index i k a) q
+  start := dfa.start
+  output := dfa.output
+}
+
+theorem collapse_transFrom (dfa : DFA (Fin (n + 1) → α) state) (i : Fin (n + 1)) (k: Fin n) (l : List (Fin n → α))
+  : dfa.transFrom (l.map (recover_index i k)) = (collapse i k dfa).transFrom l := by
+  induction l
+  case nil =>
+    simp_all only [List.map_nil]
+    rfl
+  case cons x xs ih =>
+    simp_all only [collapse, DFAO.transFrom]
+
+theorem collapse_evalFrom (dfa : DFA (Fin (n + 1) → α) state) (i : Fin (n + 1)) (k: Fin n) (l : List (Fin n → α)) (s : state)
+  : dfa.evalFrom (l.map (recover_index i k)) s = (collapse i k dfa).evalFrom l s := by
+  simp only [DFAO.evalFrom, collapse_transFrom]
+  rfl
+
+theorem collapse_eval (dfa : DFA (Fin (n + 1) → α) state) (i : Fin (n + 1)) (k: Fin n) (l : List (Fin n → α))
+  : dfa.eval (l.map (recover_index i k)) = (collapse i k dfa).eval l := collapse_evalFrom dfa i k l dfa.start
+
+theorem collapse_correct (dfa : DFA (Fin (n + 1) → Fin (b + 2)) state) (l : List ℕ) (i : Fin (n + 1)) (k: Fin n)  (hlLen : l.length = n + 1) (hl : l[i] = l[k]) (hik : i.val > k.val) :
+  dfa.eval (inputToBase (b + 2) (by omega) l (hlLen)) = (collapse i k dfa).eval (((inputToBase (b + 2) (by omega) l (hlLen))).map (remove_index i)) := by
+  rw[← collapse_eval]
+  congr
+
+  have := @eqInput_if_equal (n+1) (b) l hlLen ⟨i, by omega⟩ ⟨k, by omega⟩ hl
+
+  simp only [List.map_map]
+  suffices : ∀ v ∈ (inputToBase (b + 2) _ l hlLen), (recover_index i k ∘ remove_index i) v = v
+  .
+    ext j v
+    constructor
+    . intro h
+      simp_all
+      apply this
+      exact List.getElem?_mem h
+    . intro h
+      simp_all
+      rcases h with ⟨v', ⟨h₁, h₂⟩⟩
+      rw[h₁, ← this v', h₂]
+      . exact List.getElem?_mem h₁
+
+  intro v hv
+  dsimp
+  rw[recover_remove]
+  specialize this v hv
+  .
+    simp_all only [Fin.getElem_fin, gt_iff_lt, Fin.eta, Fin.coe_eq_castSucc]
+    ext : 1
+    simp_all only
+    rfl
+  . exact hik
+
+
+#check @dcast
