Automata/Equality_Gen.lean
@@ -1,0 +1,261 @@
+import Mathlib.Tactic
+import Mathlib.Data.List.Basic
+import Automata.DFA
+import Automata.NFA
+import Automata.Input
+import Automata.Boolean
+import Automata.Vector
+import Automata.Replicate
+import Mathlib.Data.Nat.Digits
+
+--An Auxillary theorem for left to right
+theorem eqZipOfIndexEq (lsLength : ℕ) (lss: List (List ℕ))
+      (hlb: ∀ x ∈ lss, ∀ y ∈ x, y < b) (hlss: lss.length = l) (m n : Fin l)
+      (hls: ∀ ls ∈ lss, ls.length = lsLength) (hIndexEq: ∀i, ∀ (hi : i < lsLength), lss[m][i]'(by
+        have: lss[m] ∈ lss := by
+          apply List.getElem_mem
+        rw[hls lss[m] this]
+        exact hi
+      ) = lss[n][i]'(by
+        have: lss[n] ∈ lss := by
+          apply List.getElem_mem
+        rw[hls lss[n] this]
+        exact hi
+      )): ∀ f ∈ (zipToAlphabetFin lsLength l lss hlb hlss hls), (f m).val = f n:= by
+      intro f hf
+      induction lsLength generalizing lss
+      case zero =>
+        simp only [zipToAlphabetFin, List.not_mem_nil] at hf
+      case succ lsLength ih =>
+        simp only [zipToAlphabetFin, Fin.getElem_fin, List.mem_cons] at hf
+        rcases hf with hf | hf
+        . specialize hIndexEq 0 (by norm_num)
+          simp[hf, hIndexEq]
+          exact hIndexEq
+        . apply ih (List.map (fun ls ↦ ls.tail) lss)
+          . intro i hi
+            simp only [Fin.getElem_fin, List.getElem_map]
+            rw[List.getElem_tail, List.getElem_tail]
+            apply hIndexEq
+            simp only [add_lt_add_iff_right]
+            exact hi
+          . exact hf
+
+theorem eqInput_if_equal (input : List ℕ) (hl: input.length = l) (m n : Fin l) :
+  input[m] = input[n] →  ∀ f ∈ inputToBase (b + 2) (by omega) input hl, (f m).val = (f n) := by
+    intro h
+    have stretchLenLen_aux : (stretchLen (mapToBase (b+2) input)).length = (mapToBase (b+2) input).length :=
+      stretchLen_length (mapToBase (b+2) input)
+
+    have stretchLenLen : (stretchLen (mapToBase (b+2) input)).length = input.length := by
+      simp only [stretchLenLen_aux, mapToBase_length]
+
+    have stretchLenEq: (stretchLen (mapToBase (b+2) input))[m] =
+    (stretchLen (mapToBase (b+2) input))[n] := by
+      simp_all[stretchLen, mapToBase, h]
+
+    have indexValid0 : m < (stretchLen (mapToBase (b+2) input)).length := by
+      simp [stretchLenLen]
+      omega
+
+    have indexValid1 : n < (stretchLen (mapToBase (b+2) input)).length := by
+      simp [stretchLenLen]
+      omega
+
+    have lenStretchLen0 : (stretchLen (mapToBase (b+2) input))[m].length = maxLen (mapToBase (b+2) input) := by
+      apply stretchLen_uniform
+      exact List.getElem_mem (stretchLen (mapToBase (b+2) input)) m indexValid0
+
+    have lenStretchLen1 : (stretchLen (mapToBase (b+2) input))[n].length = maxLen (mapToBase (b+2) input) := by
+      apply stretchLen_uniform
+      exact List.getElem_mem (stretchLen (mapToBase (b+2) input)) n indexValid1
+
+    have stretchLenIndexEq (i: ℕ)(hi: i < (maxLen (mapToBase (b+2) input))): (stretchLen (mapToBase (b+2) input))[m][i] = (stretchLen (mapToBase (b+2) input))[n][i] := by
+      simp only [stretchLenEq]
+
+    intro f hf
+    rw[inputToBase] at hf
+    apply eqZipOfIndexEq (maxLen (mapToBase (b+2) input)) (stretchLen (mapToBase (b+2) input))
+    . apply stretchLenIndexEq
+    . exact hf
+
+--Right to left
+theorem equal_if_toBaseEq: toBase b m = toBase b n → m = n := by
+  intro h
+  rw[← ofBase_toBase b n, ← ofBase_toBase b m]
+  congr
+
+theorem equal_if_mapToBaseEq (input: List ℕ) (m n : Fin input.length) :
+  (mapToBase (b+2) input)[m]'(by simp[mapToBase]) = (mapToBase (b+2) input)[n]'(by simp[mapToBase]) → input[m] = input[n] := by
+  intro h
+  simp only [mapToBase, List.map_cons, List.map_nil, List.getElem_cons_zero,
+    List.getElem_cons_succ] at h
+
+  apply equal_if_toBaseEq
+  simp_all only [Fin.getElem_fin, List.getElem_map]
+  exact h
+
+theorem eq_if_addZeroesEq_nonzero (n: ℕ) (L: List (List ℕ)) (k l: Fin L.length) (hn: n ≥ maxLen L)  (lenk :0 < L[k].length) (hk: L[k][0] ≠ 0) (lenl :0 < L[l].length) (hl: L[l][0] ≠ 0) :
+  addZeroes (n - L[k].length) L[k] = addZeroes (n - L[l].length) L[l] → L[k] = L[l] := by
+  intro h
+  simp only [maxLen, zero_le, max_eq_left, ge_iff_le, max_le_iff] at hn
+  have kLen: L[k].length ≤ n := by
+    trans maxLen L
+    apply len_le_maxLen
+    apply List.getElem_mem
+    exact hn
+  have lLen: L[l].length ≤ n := by
+    trans maxLen L
+    apply len_le_maxLen
+    apply List.getElem_mem
+    exact hn
+
+  have hL: n - L[k].length = n - L[l].length := by
+    by_contra hL
+    have hLen: n - L[k].length < n - L[l].length ∨ n - L[k].length > n - L[l].length := by
+      exact Nat.lt_or_gt_of_ne hL
+    have kAddLen: (addZeroes (n - L[k].length) L[k]).length = n := by simp only [addZeroesLength]; omega
+    have lAddLen: (addZeroes (n - L[l].length) L[l]).length = n :=  by simp only [addZeroesLength]; omega
+    rcases hLen with (hLen | hLen)
+    .
+      have addl : (addZeroes (n - L[l].length) L[l])[n-L[k].length] = 0 := by
+        simp[addZeroes]
+        apply List.getElem_of_replicate_append_left
+        exact hLen
+
+      have addk : (addZeroes (n - L[k].length) L[k])[n - L[k].length] ≠  0 := by
+        simp[addZeroes]
+        rw[List.getElem_append_right]
+        simp only [List.length_replicate, le_refl, tsub_eq_zero_of_le]
+        exact hk
+        . simp[*]
+        . simp_all only [Fin.getElem_fin, ne_eq, List.length_replicate, le_refl, tsub_eq_zero_of_le]
+          exact lenk
+      simp_all only [ne_eq, ge_iff_le, not_true_eq_false]
+
+    .
+      have addk : (addZeroes (n - L[k].length) L[k])[n-L[l].length] = 0 := by
+        simp[addZeroes]
+        apply List.getElem_of_replicate_append_left
+        exact hLen
+      have addl : (addZeroes (n - L[l].length) L[l])[n-L[l].length] ≠  0 := by
+        simp only [addZeroes, ne_eq]
+        rw[List.getElem_append_right]
+        simp only [List.length_replicate, le_refl, tsub_eq_zero_of_le]
+        exact hl
+        . simp only [List.length_replicate, lt_self_iff_false, not_false_eq_true]
+        . simp only [List.length_replicate, le_refl, tsub_eq_zero_of_le, lenl]
+
+      simp_all only [ge_iff_le, ne_eq]
+  rw[← hL] at h
+  simp only [addZeroes, List.append_cancel_left_eq] at h
+  exact h
+
+theorem contra (input : List ℕ) (m n : Fin input.length) (h : (stretchLen (mapToBase (b+2) input))[m]'(by simp[stretchLen_length, mapToBase_length]) = (stretchLen (mapToBase (b+2) input))[n]'(by simp[stretchLen_length, mapToBase_length])) (hn: input[n.val] = 0) (hm : input[m.val] ≠ 0) : False := by
+  simp[stretchLen, mapToBase, toBase, hn] at h
+  have : ∀ x ∈ addZeroes (maxLen (List.map (toBase (b + 2)) input)) [], x = 0 ∨ x ∈ [] := by
+    apply addZeroes_elem
+  simp only [List.not_mem_nil, or_false] at this
+  rw[← h] at this
+  have hbm: ∀x ∈ (toBase (b+2) input[m]), x = 0 := by
+    intro x hx
+    apply this
+    simp only [addZeroes, le_add_iff_nonneg_left, zero_le, List.mem_append, List.mem_replicate,
+      ne_eq, List.mem_reverse]
+    right
+    exact List.mem_reverse.mp hx
+  have: input[m] > 0 := by exact Nat.zero_lt_of_ne_zero hm
+  have hPos := toBase_lead_nonzero (b+2) input[m] (by omega) this
+  specialize hbm ((toBase (b+2) input[m])[0]'(by
+      apply toBase_len_nonzero <;> omega
+  ))
+  have hyp : (toBase (b+2) input[m])[0]'(by
+  have:= toBase_len_nonzero (b+2) input[m] (by omega) (by omega)
+  omega) ∈ toBase (b+2) input[m] := by apply List.getElem_mem
+  specialize hbm hyp
+  rw[hbm] at hPos
+  contradiction
+
+theorem eq_if_stretchLenEq (input : List ℕ) (m n : Fin input.length) :
+  (stretchLen (mapToBase (b+2) input))[m]'(by simp[stretchLen_length, mapToBase_length]) = (stretchLen (mapToBase (b+2) input))[n]'(by simp[stretchLen_length, mapToBase_length]) → input[m] = input[n] := by
+  intro h
+  apply equal_if_mapToBaseEq
+  by_cases hm: input[m.val] = 0
+  . by_cases hn : input[n.val] = 0
+    . simp[mapToBase, hn, hm]
+    . by_contra; apply contra; exact h.symm; exact hm; exact hn
+  by_cases hn: input[n.val] = 0
+  . by_contra; apply contra; exact h; exact hn; exact hm
+  apply eq_if_addZeroesEq_nonzero (maxLen (mapToBase (b+2) input)) (mapToBase (b+2) input) ⟨m, by simp[mapToBase]⟩ ⟨n, by simp[mapToBase_length]⟩
+  . simp only [ge_iff_le]; rfl
+  . simp only [mapToBase, List.map_cons, List.map_nil, List.getElem_cons_zero, ne_eq]
+    refine Nat.ne_zero_iff_zero_lt.mpr ?_
+    simp only [Fin.getElem_fin, List.getElem_map]
+    apply toBase_lead_nonzero
+    simp_all only [Fin.getElem_fin, ge_iff_le, le_add_iff_nonneg_left, zero_le]
+    . omega
+  . simp only [mapToBase, List.map_cons, List.map_nil, List.getElem_cons_zero, ne_eq]
+    refine Nat.ne_zero_iff_zero_lt.mpr ?_
+    simp only [Fin.getElem_fin, List.getElem_map]
+    apply toBase_lead_nonzero
+    simp_all only [Fin.getElem_fin, ge_iff_le, le_add_iff_nonneg_left, zero_le]
+    . omega
+  . simp_all[stretchLen]
+  . simp only [mapToBase, Fin.getElem_fin, List.getElem_map]
+    apply toBase_len_nonzero <;> omega
+  . simp only [mapToBase, Fin.getElem_fin, List.getElem_map]
+    apply toBase_len_nonzero <;> omega
+
+
+
+
+theorem indexEqOfEqZip (b lsLength : ℕ) (lss: List (List ℕ))
+      (hlb: ∀ x ∈ lss, ∀ y ∈ x, y < b) (hlss: lss.length = 2)
+      (hls: ∀ ls ∈ lss, ls.length = lsLength) :
+      (∀ f ∈ (zipToAlphabetFin lsLength 2 lss hlb hlss hls), (f 0).val = f 1)
+      → ∀i, ∀ hi : i < lsLength, lss[0][i]'(by
+        have: lss[0] ∈ lss := by
+          apply List.getElem_mem
+        rw[hls lss[0] this]
+        exact hi
+      ) = lss[1][i]'(by
+        have: lss[1] ∈ lss := by
+          apply List.getElem_mem
+        rw[hls lss[1] this]
+        exact hi
+      ) := by
+        intro h
+        induction lsLength generalizing lss
+        case zero => intro i hi; contradiction
+        case succ m ih =>
+          intro i hi
+          simp only [zipToAlphabetFin, Fin.getElem_fin, List.mem_cons, Fin.isValue,
+            forall_eq_or_imp, Fin.val_zero, Fin.val_one] at h
+          rcases h with ⟨h1, h2⟩
+          specialize ih (List.map (fun ls ↦ ls.tail) lss)
+          specialize ih (zipTailHlb lss hlb)
+          specialize ih (zipTailHlss 2 lss hlss)
+          specialize ih (zipTailHls lss hls)
+          specialize ih h2
+          simp at ih
+          have lss0 : lss[0] ∈ lss := by apply List.getElem_mem lss 0 _
+          have lss1 : lss[1] ∈ lss := by apply List.getElem_mem
+          have i0Len : i < lss[0].length := by
+            specialize hls lss[0]
+            specialize hls lss0
+            rwa [hls]
+          have i1Len : i < lss[1].length := by
+            specialize hls lss[1]
+            specialize hls lss1
+            rwa [hls]
+          match i with
+          | 0 => exact h1
+          | n + 1 =>
+            simp only [add_lt_add_iff_right] at hi
+            specialize ih n hi
+            -- rw[← tailIndex lss[0] n i0Len]
+            -- rw[← tailIndex lss[1] n i1Len]
+            simp only [List.getElem_tail, *] at ih
+            exact ih
+
+-- theorem equal_if_eqInput
